generate.sh
@@ -18,9 +18,11 @@ zip -r code.zip example-code
 popd
 
 echo "Collecting generated HTML..."
-mkdir out
+mkdir -p out
 cp -r blog/_site out/blog
 cp -r package-docs/manual/_out/html-multi out/package-docs
 cp -r textbook/_out/html-multi out/textbook
 cp textbook/_out/code.zip out/textbook/
 
+echo "The sites can be viewed by running a server. If in doubt, try the following command:"
+echo "python3 ./serve.py 8000"
